DNS patched for BoundedIndex Merge.

src/Examples/DnsServer/Dns.v
@@ -8,12 +8,11 @@ Require Import Fiat.QueryStructure.Automation.AutoDB
         Fiat.QueryStructure.Implementation.DataStructures.BagADT.BagADT
         Fiat.QueryStructure.Automation.IndexSelection
         Fiat.QueryStructure.Specification.SearchTerms.ListPrefix
-        Fiat.QueryStructure.Automation.SearchTerms.FindSuffixSearchTerms
+        Fiat.QueryStructure.Automation.SearchTerms.FindPrefixSearchTerms
         Fiat.QueryStructure.Automation.QSImplementation
         Fiat.Examples.DnsServer.packet
         Fiat.Examples.DnsServer.DnsSchema
         Fiat.Examples.DnsServer.DnsLemmas.
-
 
 Definition DnsSig : ADTSig :=
   ADTsignature {
@@ -26,15 +25,15 @@ Definition DnsSpec : ADT DnsSig :=
   QueryADTRep DnsSchema {
     Def Constructor "Init" (_ : unit) : rep := empty,
 
-    update "AddData" (t : DNSRRecord) : bool :=
-      Insert t into sCOLLECTIONS,
+    update "AddData" (this : rep, t : DNSRRecord) : bool :=
+      Insert t into this!sCOLLECTIONS,
 
-    query "Process" (p : packet) : packet :=
+    query "Process" (this : rep, p : packet) : packet :=
       let t := qtype (questions p) in
       Repeat 1 initializing n with qname (questions p)
                defaulting rec with (ret (buildempty p))
-         {{ rs <- For (r in sCOLLECTIONS)      (* Bind a list of all the DNS entries *)
-                  Where (IsSuffix n r!sNAME) (* prefixed with [n] to [rs] *)
+         {{ rs <- For (r in this!sCOLLECTIONS)      (* Bind a list of all the DNS entries *)
+                  Where (IsPrefix r!sNAME n) (* prefixed with [n] to [rs] *)
                   (* prefix: "com.google" is a prefix of "com.google.scholar" *)
                   Return r;
             If (negb (is_empty rs))        (* Are there any matching records? *)
@@ -56,7 +55,7 @@ Definition DnsSpec : ADT DnsSig :=
                 (* multiple matches -- add them all as answers in the packet *)
                   ret (List.fold_left addan bfrs (buildempty p))
               else              (* prefix but record's QNAME not an exact match *)
-                (* return all the prefix records that are nameserver records -- 
+                (* return all the prefix records that are nameserver records --
                  ask the authoritative servers *) (* TODO does this return one, or return all? *)
                 bfrs' <- [[x in bfrs | x!sTYPE = NS]];
                 ret (List.fold_left addns bfrs' (buildempty p))
@@ -69,28 +68,44 @@ Definition DnsSpec : ADT DnsSig :=
 
 (* implement the DNS record constraint check as code that counts the number of occurrences of
 the constraint being broken (refines the boolean x1 in AddData) *)
+
+Notation "( x 'in' r '!' Ridx ) bod" :=
+  (let qs_schema : QueryStructureSchema := _ in
+   let r' : UnConstrQueryStructure qs_schema := r in
+   let Ridx' := ibound (indexb (@Build_BoundedIndex _ _ (QSschemaNames qs_schema) Ridx%string _)) in
+   @UnConstrQuery_In _ qs_schema r' Ridx'
+            (fun x : @RawTuple (GetNRelSchemaHeading (qschemaSchemas qs_schema) Ridx') => bod)) : QueryImpl_scope.
+
+Definition GetAttributeRawBnd {heading : Heading}
+           (tup : @RawTuple heading)
+           (idx : (BoundedIndex (HeadingNames heading)))
+  : Domain heading (ibound (indexb idx)) :=
+  GetAttributeRaw tup (ibound (indexb idx)).
+
+Notation "tup '!' idx" := (GetAttributeRaw tup ``idx) : TupleImpl_scope.
+
 Lemma refine_count_constraint_broken :
   forall (n : DNSRRecord) (r : UnConstrQueryStructure DnsSchema),
     refine {b |
             decides b
-                    (forall tup' : @IndexedTuple (GetHeading DnsSchema sCOLLECTIONS),
+                    (forall tup' : @IndexedRawTuple (GetHeading DnsSchema sCOLLECTIONS),
                        (r!sCOLLECTIONS)%QueryImpl tup' ->
                        n!sNAME = (indexedElement tup')!sNAME -> n!sTYPE <> CNAME)}
            (If (beq_RRecordType n!sTYPE CNAME)
                Then count <- Count
-               For (UnConstrQuery_In r ``(sCOLLECTIONS)
-                                     (fun tup : Tuple =>
-                                        Where (n!sNAME = tup!sNAME)
-                                              Return tup ));
-            ret (beq_nat count 0) Else ret true).
+               For (tup in r!sCOLLECTIONS)
+               (Where (n!sNAME = GetAttributeRawBnd tup ``sNAME)
+                      Return tup )%QueryImpl;
+    ret (beq_nat count 0) Else ret true).
 Proof.
   intros; setoid_rewrite refine_pick_decides at 1;
   [ | apply refine_is_CNAME__forall_to_exists | apply refine_not_CNAME__independent ].
   (* refine existence check into query. *)
+
   match goal with
       |- context[{b | decides b
                               (exists tup : @IndexedTuple ?heading,
-                                 (@GetUnConstrRelation ?qs_schema ?qs ?tbl tup /\ @?P tup))}]
+                                 (@GetUnConstrRelationBnd ?qs_schema ?qs ?tbl tup /\ @?P tup))}]
       =>
       let H1 := fresh in
       let H2 := fresh in
@@ -106,12 +121,12 @@ Proof.
                      |
                      assert (DecideableEnsemble P') as H2;
                        [ simpl; eauto with typeclass_instances (* Discharge DecideableEnsemble w/ intances. *)
-                       | setoid_rewrite (@refine_constraint_check_into_query' qs_schema tbl qs P P' H2 H1); clear H1 H2 ] ]) end.
+                       | setoid_rewrite (@refine_constraint_check_into_query' qs_schema (ibound (indexb tbl)) qs P P' H2 H1); clear H2 H1 ] ]) end.
   remember n!sTYPE; refine pick val (beq_RRecordType d CNAME); subst;
   [ | case_eq (beq_RRecordType n!sTYPE CNAME); intros;
       rewrite <- beq_RRecordType_dec in H; find_if_inside;
       unfold not; simpl in *; try congruence ].
-  simplify with monad laws.
+  intros; simplify with monad laws; simpl.
   autorewrite with monad laws.
   setoid_rewrite negb_involutive.
   reflexivity.
@@ -120,7 +135,7 @@ Qed.
 (* -------------------------------------------------------------------------------------- *)
 
 Theorem DnsManual :
-  MostlySharpened DnsSpec.
+  FullySharpened DnsSpec.
 Proof.
 
   (* the two components here (start honing + GenerateIndexesForAll) are manual versions of
@@ -156,11 +171,11 @@ start sharpening ADT. {
     etransitivity.
     Check refine_bind.
     (* implement decision procedure *)
-    { 
+    {
       apply refine_bind;
       [ apply refine_check_one_longest_prefix_s
       | intro; higher_order_reflexivity ].
-      intros. clear H. clear H1. unfold get_name. 
+      intros. clear H. clear H1. unfold get_name.
       eapply For_computes_to_In in H0.
       inv H0.
       - apply H.
@@ -172,11 +187,11 @@ start sharpening ADT. {
     apply refine_If_Then_Else.
     etransitivity.
     { (* Locate "unique". *)
-      
+
       (* setoid_rewrite refine_check_one_longest_prefix_CNAME. *)
       (* simplify with monad laws. *)
       (* reflexivity. *)
-      
+
       apply refine_bind;        (* rewrite instead of apply *)
       [ eapply refine_check_one_longest_prefix_CNAME | intro; higher_order_reflexivity ].
 
@@ -185,19 +200,19 @@ start sharpening ADT. {
       - eapply tuples_in_relation_satisfy_constraint_specific.
         Check refine_check_one_longest_prefix_CNAME. apply H0.
       (* exciting! *)
-      -                        
+      -
         clear H.
         intros.
-        instantiate (1 := (qname (questions n))). 
+        instantiate (1 := (qname (questions n))).
         eapply For_computes_to_In in H0.
-        inv H0. unfold IsSuffix in *. unfold get_name.
+        inv H0. unfold get_name.
       + apply H2.
       + pose proof IsSuffix_string_dec. intros. auto.
       + auto.
     }
     simplify with monad laws.
     reflexivity. reflexivity.
-    
+
     reflexivity. subst H1; reflexivity.
     unfold pointwise_relation; intros; higher_order_reflexivity.
     finish honing. finish honing.
@@ -217,7 +232,7 @@ start sharpening ADT. {
     (* x1 = check constraint between n (the record) and every other tuple  *)
     (* x2 = check constraint between every other tuple and n (the record) *)
     (* differs in the final step ((_)!sTYPE <> CNAME) *)
-    
+
     (* redundant *)
     (* subst_all. *)
     (* match goal with *)
@@ -237,10 +252,8 @@ start sharpening ADT. {
     apply refine_If_Then_Else.
     -
       (* simplify with monad laws. *)
-      Check refine_under_bind.
       apply refine_under_bind; intros.
-      (* apply refine_under_bind; intros. *) 
-      Check refine_Count.
+      (* apply refine_under_bind; intros. *)
       setoid_rewrite refine_Count. simplify with monad laws.
       apply refine_under_bind.  Check refine_under_bind. intros.
       setoid_rewrite refine_subcheck_to_filter; eauto.
@@ -249,8 +262,10 @@ start sharpening ADT. {
       simplify with monad laws.
       Check clear_nested_if.
       rewrite clear_nested_if by apply filter_nil_is_nil.
+      (* Need to replace if with If for implement_bag_methods to work. *)
+      set_evars; setoid_rewrite refine_if_If.
       higher_order_1_reflexivity.
-      (* clears goal, but H1 is still in the context, and it still has the 
+      (* clears goal, but H1 is still in the context, and it still has the
          For/Where/Return ~> _ unimplemented *)
       eauto with typeclass_instances.
     - simplify with monad laws.
@@ -261,21 +276,25 @@ start sharpening ADT. {
       (* why is this OK? it didn't get rid of x0 nondeterminism *)
       reflexivity.
     (* - finish honing. *)
-  } 
+  }
   (* higher level of reasoning *)
 
   GenerateIndexesForAll         (* ? in IndexSelection, see GenerateIndexesFor *)
   (* specifies that you want to use the suffix index structure TODO *)
-  ltac:(CombineCase2 matchFindSuffixIndex matchEqIndex)
-         ltac:(fun attrlist => make simple indexes using attrlist).
+  ltac:(CombineCase3 matchFindPrefixIndex matchEqIndex)
+         ltac:(fun attrlist =>
+  make_simple_indexes
+    attrlist
+    ltac:(CombineCase6 BuildEarlyFindPrefixIndex ltac:(LastCombineCase6 BuildEarlyEqualityIndex))
+           ltac:(CombineCase5 BuildLastFindSuffixIndex ltac:(LastCombineCase5 BuildLastEqualityIndex))).
   (* SearchTerm and SearchUpdateTerm: efficiently do quality test on the name columns *)
-  (* it figures out what data structure to use *)
+  (* it figures out what datac structure to use *)
   (* BagMatchSearchTerm *)
   (* implement query as calls to abstract bag find function *)
   (* then plug in data structures that impl bag find (chooses b/t them?) *)
 
   (* hone constructor "Init". *)
-  { 
+  {
     simplify with monad laws.
     rewrite refine_QSEmptySpec_Initialize_IndexedQueryStructure.
     finish honing.
@@ -290,12 +309,12 @@ start sharpening ADT. {
     - apply refine_If_Then_Else.
       + simplify with monad laws.
         implement_Query
-          ltac:(CombineCase5 SuffixIndexUse EqIndexUse)
-                 ltac:(CombineCase10 createEarlySuffixTerm createEarlyEqualityTerm)
-                        ltac:(CombineCase7 createLastSuffixTerm createLastEqualityTerm)
-                               ltac:(CombineCase7 SuffixIndexUse_dep EqIndexUse_dep)
-                        ltac:(CombineCase11 createEarlySuffixTerm_dep createEarlyEqualityTerm_dep)
-                        ltac:(CombineCase8 createLastSuffixTerm_dep createLastEqualityTerm_dep).
+          ltac:(CombineCase5 PrefixIndexUse EqIndexUse)
+                 ltac:(CombineCase10 createEarlyPrefixTerm createEarlyEqualityTerm)
+                        ltac:(CombineCase7 createLastPrefixTerm createLastEqualityTerm)
+                               ltac:(CombineCase7 PrefixIndexUse_dep EqIndexUse_dep)
+                        ltac:(CombineCase11 createEarlyPrefixTerm_dep createEarlyEqualityTerm_dep)
+                        ltac:(CombineCase8 createLastPrefixTerm_dep createLastEqualityTerm_dep).
         simplify with monad laws.
         rewrite (@refineEquiv_swap_bind nat).
         setoid_rewrite refine_if_If.
@@ -304,30 +323,29 @@ start sharpening ADT. {
         reflexivity.
       + simplify with monad laws.
         implement_Query
-          ltac:(CombineCase5 SuffixIndexUse EqIndexUse)
-                 ltac:(CombineCase10 createEarlySuffixTerm createEarlyEqualityTerm)
-                        ltac:(CombineCase7 createLastSuffixTerm createLastEqualityTerm)
-                               ltac:(CombineCase7 SuffixIndexUse_dep EqIndexUse_dep)
-                                      ltac:(CombineCase11 createEarlySuffixTerm_dep createEarlyEqualityTerm_dep)
-                                             ltac:(CombineCase8 createLastSuffixTerm_dep createLastEqualityTerm_dep).
-        simplify with monad laws. 
+          ltac:(CombineCase5 PrefixIndexUse EqIndexUse)
+                 ltac:(CombineCase10 createEarlyPrefixTerm createEarlyEqualityTerm)
+                        ltac:(CombineCase7 createLastPrefixTerm createLastEqualityTerm)
+                               ltac:(CombineCase7 PrefixIndexUse_dep EqIndexUse_dep)
+                                      ltac:(CombineCase11 createEarlyPrefixTerm_dep createEarlyEqualityTerm_dep)
+                                             ltac:(CombineCase8 createLastPrefixTerm_dep createLastEqualityTerm_dep).
+        simplify with monad laws.
         rewrite (@refineEquiv_swap_bind nat).
         setoid_rewrite refine_if_If.
         implement_Insert_branches.
         reflexivity.
     - reflexivity.              (* seems fully deterministic here *)
     - finish honing.
-    }
-
+  }
   (* hone method "Process". *) {
     simplify with monad laws.
     implement_Query             (* in AutoDB, implement_Query' has steps *)
-      ltac:(CombineCase5 SuffixIndexUse EqIndexUse)
-             ltac:(CombineCase10 createEarlySuffixTerm createEarlyEqualityTerm)
-                    ltac:(CombineCase7 createLastSuffixTerm createLastEqualityTerm)
-                           ltac:(CombineCase7 SuffixIndexUse_dep EqIndexUse_dep)
-                                  ltac:(CombineCase11 createEarlySuffixTerm_dep createEarlyEqualityTerm_dep)
-                                         ltac:(CombineCase8 createLastSuffixTerm_dep createLastEqualityTerm_dep).
+      ltac:(CombineCase5 PrefixIndexUse EqIndexUse)
+             ltac:(CombineCase10 createEarlyPrefixTerm createEarlyEqualityTerm)
+                    ltac:(CombineCase7 createLastPrefixTerm createLastEqualityTerm)
+                           ltac:(CombineCase7 PrefixIndexUse_dep EqIndexUse_dep)
+                                  ltac:(CombineCase11 createEarlyPrefixTerm_dep createEarlyEqualityTerm_dep)
+                                         ltac:(CombineCase8 createLastPrefixTerm_dep createLastEqualityTerm_dep).
     simplify with monad laws.
     simpl.
     setoid_rewrite (refine_pick_val _ H).
@@ -335,68 +353,28 @@ start sharpening ADT. {
     setoid_rewrite (@refine_filtered_list _ _ _ _).
     finish honing.
   }
-  
-  FullySharpenQueryStructure' DnsSchema Index.
-  (* implement_bag_methods needs to be patched for this goal. *)
+  pose_headings_all.
+  FullySharpenQueryStructure DnsSchema Index.
+}
 
-  - implement_bag_methods.
-  - implement_bag_methods.
+{ simpl; pose_string_ids; pose_headings_all;
+  pose_search_term;  pose_SearchUpdateTerms.
+  unfold name in *.
+  BuildQSIndexedBags'
+  ltac:(CombineCase6 BuildEarlyTrieBag BuildEarlyEqualityBag)
+         ltac:(CombineCase5 BuildLastTrieBag BuildLastEqualityBag). }
+
+{ cbv zeta; pose_string_ids; pose_headings_all;
+    pose_search_term;  pose_SearchUpdateTerms;
+    simpl Sharpened_Implementation;
+    unfold
+      Update_Build_IndexedQueryStructure_Impl_cRep,
+    Join_Comp_Lists',
+    GetIndexedQueryStructureRelation,
+    GetAttributeRaw; simpl;
+    higher_order_reflexivityT. }
+
 Time Defined.
 
-    Definition DnsDelegateReps
-    : ilist (fun ns => Type) (qschemaSchemas DnsSchema).
-      simpl; econstructor; [ | econstructor ].
-      exact (list (@Tuple
-           <sNAME :: name, sTYPE :: RRecordType, sCLASS :: RRecordClass,
-              sTTL :: nat, sDATA :: string>%Heading)).
-    Defined.
-
-    Definition DnsDelegateSearchUpdateTerms
-    : ilist (fun ns => SearchUpdateTerms (schemaHeading (relSchema ns)))
-             (qschemaSchemas DnsSchema).
-      simpl; econstructor; [ | econstructor ].
-      exact  DnsSearchUpdateTerm.
-    Defined.
-
-
-
-    Definition DnsDelegateImpls
-    : i2list2 (fun ns (SearchTerm : SearchUpdateTerms (schemaHeading (relSchema ns)))
-                   (Rep : Type) =>
-                 ComputationalADT.pcADT
-                   (BagSig (@Tuple (schemaHeading (relSchema ns)))
-                           (BagSearchTermType SearchTerm)
-                           (BagUpdateTermType SearchTerm))
-                   Rep)
-              DnsDelegateSearchUpdateTerms
-              DnsDelegateReps.
-      simpl; econstructor; [ | econstructor ].
-      let p := eval simpl in (projT2 (BagADTImpl (fun _ => true)
-                         (@ListAsBag
-                            _
-                            (BagSearchTermType DnsSearchUpdateTerm)
-                            (BagUpdateTermType DnsSearchUpdateTerm)
-                            {| pst_name := nil;
-                               pst_filter := fun _ => true |}
-                            (BagMatchSearchTerm DnsSearchUpdateTerm)
-                            (BagApplyUpdateTerm DnsSearchUpdateTerm) ))) in
-          exact p.
-    Defined.
-
-    Definition DnsImpl : SharpenedUnderDelegates DnsSig.
-      Time let
-          Impl := eval simpl in (projT1 DnsManual) in exact Impl.
-    Defined.
-
-    Print DnsImpl.
-    Definition ExtractWorthyDNSImpl : ComputationalADT.cADT DnsSig.
-      let s := eval unfold DnsImpl in DnsImpl in
-          let Impl := eval simpl in
-          (Sharpened_Implementation s
-                                    (LookupQSDelegateReps DnsDelegateReps)
-                                    (LookupQSDelegateImpls DnsDelegateImpls)) in exact Impl.
-    Defined.
-
-    Print ExtractWorthyDNSImpl.
-
-    Extraction "bar.ml" ExtractWorthyDNSImpl.
+Time Definition DNSImpl := Eval simpl in (projT1 DnsManual).
+Print DNSImpl.
