src/ADTRefinement/GeneralBuildADTRefinements.v
@@ -670,9 +670,9 @@ Tactic Notation "finish" "sharpening" constr(delegatees):=
 
 Tactic Notation "finish" "honing" :=
   match goal with
-    | |- ?R _ (?H _ ) =>
-      try subst H; higher_order_reflexivity
     | |- ?R _ (?H _ _) =>
+      try subst H; higher_order_reflexivity
+    | |- ?R _ (?H _ ) =>
       try subst H; higher_order_reflexivity
   end.
 
